lakefile.lean
@@ -6,7 +6,8 @@ package «mm-lean4»
 require std from git "https://github.com/leanprover/std4" @ "main"
 
 @[default_target]
-lean_lib Metamath
+lean_lib Metamath where
+  roots := #[`Metamath, `Metamath.Translate]
 
 @[default_target]
 lean_exe «mm-lean4» where
